formal/inference/Trace_Matches.thy
@@ -1,0 +1,32 @@
+theory Trace_Matches
+imports Inference
+begin
+datatype io = I | O
+type_synonym index = "nat \<times> io \<times> nat"
+
+fun lookup :: "index \<Rightarrow> execution \<Rightarrow> value" where
+  "lookup (eventNo, I, inx) t = (let (_, inputs, _) = nth t eventNo in nth inputs inx)" |
+  "lookup (eventNo, io.O, inx) t = (let (_, _, outputs) = nth t eventNo in nth outputs inx)"
+
+abbreviation eventNum :: "index \<Rightarrow> nat" where
+  "eventNum i \<equiv> fst i"
+
+abbreviation io :: "index \<Rightarrow> io" where
+  "io i \<equiv> fst (snd i)"
+
+abbreviation inx :: "index \<Rightarrow> nat" where
+  "inx i \<equiv> snd (snd i)"
+
+definition get_intratrace_matches :: "execution \<Rightarrow> (index \<times> index) fset" where
+  "get_intratrace_matches e = Abs_fset {(a, b). lookup a e = lookup b e \<and> eventNum a \<le> eventNum b}"
+
+primrec get_all_intratrace_matches :: "log \<Rightarrow> (index \<times> index) fset list" where
+  "get_all_intratrace_matches [] = []" |
+  "get_all_intratrace_matches (h#t) = (get_intratrace_matches h)#(get_all_intratrace_matches t)"
+
+(* 
+  To detect all intertrace matches, walk the trace in the current machine and replace eventNo with
+  the corresponding transition's uid. If the uids match then there's an intertrace match.
+*)
+
+end
